imp_system/imp/Imp.v
@@ -232,8 +232,7 @@ Section Denote.
       (if (forallb (fun v => match v with | Vint _ => true | _ => false end) eval_args) then Ret tt else triggerUB);;;
       let eval_zs := List.map (fun v => match v with | Vint z => z | _ => 0%Z end) eval_args in
       (if (forallb intrange_64 eval_zs) then Ret tt else triggerUB);;;
-      v <- trigger (IO f eval_zs↑ top1);;
-      v <- v↓?;;
+      v <- trigger (IO f eval_zs);;
       trigger (SetVar x (Vint v));;; tau;; Ret Vundef
 
     | AddrOf x X =>
