proofmode/wsim/WSimCore.v
@@ -257,15 +257,15 @@ Section WSIM.
     iIntros (? ? ?) "IST". iPoseProof ("H" with "IST") as "H". iApply "H". eauto.
   Qed.  
 
-  Lemma wsim_syscall
-    E r g {R} RR ps pt st_src st_tgt k_src k_tgt fn varg rvs
+  Lemma wsim_io
+    E r g {R} RR ps pt st_src st_tgt I O k_src k_tgt fn (varg: I)
   :
-    (∀ vret, @wsim E r g R RR true true (st_src, k_src vret) (st_tgt, k_tgt vret))
+    (∀ (vret: O), @wsim E r g R RR true true (st_src, k_src vret) (st_tgt, k_tgt vret))
   -∗
-    (wsim E r g RR ps pt (st_src, trigger (IO fn varg rvs) >>= k_src) (st_tgt, trigger (IO fn varg rvs) >>= k_tgt)).
+    (wsim E r g RR ps pt (st_src, trigger (IO fn varg) >>= k_src) (st_tgt, trigger (IO fn varg) >>= k_tgt)).
   Proof.
     unfold wsim. iIntros "H D".
-    iApply isim_syscall. iIntros. 
+    iApply isim_io. iIntros. 
     iPoseProof ("H" with "D") as "H". iFrame.
   Qed.
 
